States and post2nfa

parser/regex.dfy
@@ -1,8 +1,9 @@
 
+//based on https://swtch.com/~rsc/regexp/regexp1.html
 include "../libraries/src/Wrappers.dfy"
 module RegEx {
     import opened Wrappers
-    datatype RegexPiece = Char(value: char) | GroupStart(id: int) | GroupEnd(id: int) | Plus | Star | Optional | Alt | Concat
+    datatype RegexPiece = Char(value: char) | GroupStart(id: nat) | GroupEnd(id: nat) | Plus | Star | Optional | Alt | Concat
     datatype Paren = Paren(natom: int, nalt: int)
     function RegToChar(re: RegexPiece): char {
         match re {
@@ -25,15 +26,18 @@ module RegEx {
         var groups: seq<int> := [];
         var parens: seq<Paren> :=[];
         for i := 0 to |re| 
-
+            invariant |groups| == |parens|
         {
+            // print "char -> ";
+            // print re[i];
+            // print "\n";
             match re[i] {
                 case '(' => {
                     if natom > 1 {
                         natom := natom -1;
                         buf := buf + [Concat];
                     }
-                    parens := parens + [Paren(nalt, natom)];
+                    parens := parens + [Paren(natom, nalt)];
                     buf := buf + [GroupStart(groupid)];
                     groups := groups + [groupid];
                     groupid := groupid + 1;
@@ -44,6 +48,7 @@ module RegEx {
                     if natom == 0 {
                         return Failure("Missing atom");
                     }
+                    natom := natom - 1;
                     while natom > 0 {
                         buf := buf + [Concat];
                         natom := natom - 1;
@@ -54,6 +59,7 @@ module RegEx {
                     if |parens| == 0 || |groups| == 0 || natom == 0 {
                         return Failure("missing atom or paren");
                     }
+                    natom := natom - 1;
                     while natom > 0 {
                         buf := buf + [Concat];
                         natom := natom - 1;
@@ -69,6 +75,11 @@ module RegEx {
                     natom := natom + 1;
                     buf := buf + [GroupEnd(groups[|groups|-1])];
                     groups := groups[0..|groups|-1];
+                    // print "nalt: ";
+                    // print nalt;
+                    // print " natom: ";
+                    // print natom;
+                    // print "\n";
                 }
                 case '*' => {
                     if natom == 0 {
@@ -101,6 +112,7 @@ module RegEx {
         if |parens| != 0 {
             return Failure("Missing )");
         }
+        natom := natom - 1;
         while natom > 0 {
             buf := buf + [Concat];
             natom := natom - 1;
@@ -110,6 +122,272 @@ module RegEx {
             nalt := nalt - 1;
         }
         return Success(buf);
+    }
+    datatype MatchKind = Split | Match | Wild | MatchChar(c: char)
+    class State {
+        ghost var repr : set<object>
+        var id: nat
+        var c: MatchKind
+        var negated: bool
+        var out: State?
+        var out1: State?
+        var lastlist: nat
+        var groups: set<nat>
+        var origin: RegexPiece
+
+        constructor(id: nat, c: MatchKind, out: State?, out1: State?, negated: bool) 
+            ensures this.id == id
+            ensures this.c == c
+            ensures this.out == out
+            ensures this.out1 == out1
+            ensures this.negated == negated
+            ensures this.groups == {}
+        {
+            this.id := id;
+            this.c := c;
+            this.out := out;
+            this.out1 := out1;
+            this.negated := negated;
+            this.groups := {};
+
+        }
+        
+        ghost predicate Valid() 
+            reads this, repr, out, out1
+            decreases repr
+        {
+            this in repr &&
+            (this.out != null ==> this !in this.out.repr && this.out.repr <= repr) &&
+            (this.out1 != null ==> this !in this.out1.repr && this.out1.repr <= repr) &&
+            (this.out != null && this.out1 != null ==> this.out1.repr !! this.out.repr)
+
+        }
+    }
+    
+    datatype StateUpdate = Out(out: State) | Out1(out: State)
+    datatype FragC = FragC(start: State, out: seq<StateUpdate>)
+
+    class Frag {
+        ghost var repr: set<object>
+        var start: State
+        var out: array<StateUpdate>
+
+        constructor(start: State, out: array<StateUpdate>)
+            ensures this.start == start 
+            ensures this.out == out 
+        {
+            this.start := start;
+            this.out := out;
+        }
+
+        // ghost predicate Valid()
+        //     reads this, repr, out
+        // {
+        //     this in repr &&
+        //     start in repr &&
+        //     forall i :: 0 <= i < out.Length ==> OutSet(out[i]) in repr
+        // }
+    }
+
+    // method pop<T>(stack: seq<T>) returns (e: T)
+    //     requires |stack| > 0
+    // {
+    //     e := stack[|stack|-1];
+    //     stack:=stack[..|stack|-1];
+    // }
+    function OutSet(ls: StateUpdate): State {
+        match ls {
+            case Out(out) => out
+            case Out1(out1) => out1
+        }
+    }
+
+    function sout(s: State): State? 
+        reads s, s.out
+    {
+        s.out
+    }
+
+    function lout(s: State): State? 
+        reads s, s.out1
+    {
+        s.out1
+    }
+
+
+    // method patch(l: Frag, s: Frag)
+    //     // requires l.Valid()
+    //     modifies l.repr
+    //     modifies l.out
+    //     modifies set i | 0 <= i < |l.out[..]| :: OutSet(l.out[i])
+    //     modifies set i | 0 <= i < l.out.Length :: OutSet(l.out[i])
+    //     // modifies set i | 0 <= i < l.out.Length :: sout(OutSet(l.out[i]))
+    // {
+    //     var i:=0;
+    //     while i < l.out.Length
+    //         invariant 0 <= i <= l.out.Length
+    //     {
+    //         match l.out[i]
+    //         {
+    //             case Out(out) => {
+    //                 out.out := s.start;
+    //             }
+    //             case Out1(out) => {
+    //                 out.out1 := s.start;
+    //             }
+    //         }
+    //         i := i+1;
+    //     }
+    // }
+
+    method patch(l: FragC, s: FragC)
+        modifies set i | 0 <= i < |l.out| :: OutSet(l.out[i])
+    {
+        var i:=0;
+        while i < |l.out|
+            invariant 0 <= i <= |l.out|
+        {
+            match l.out[i]
+            {
+                case Out(out) => {
+                    out.out := s.start;
+                }
+                case Out1(out) => {
+                    out.out1 := s.start;
+                }
+            }
+            i := i+1;
+        }
+    }
+
+    method post2nfa(postfix: seq<RegexPiece>) returns (start: State)
+        ensures fresh(start)
+    {
+        expect |postfix| > 0, "postfix seq should contain an element";
+        var stack: seq<FragC> := [];
+        var groups: map<nat, (nat, nat)> := map[];
+        var states: seq<State?> := [];
+        var sid := 1;
+        for i:=0 to |postfix| 
+            invariant forall frag :: frag in stack ==> fresh(frag.start)
+            invariant forall state :: state !=null && state in states ==> fresh(state)
+            invariant |states| == i
+        {
+            match postfix[i] {
+                case Char(c) => {
+                    var s := new State(sid, MatchChar(c), null, null, false);
+                    sid := sid+1;
+                    s.origin := postfix[i];
+                    states := states +[s];
+                    stack := stack +[FragC(s,[Out(s)])];
+                }
+                case GroupStart(id) => {
+                    groups := groups[id := (i+1,0)];
+                    states := states +[null];
+                }
+                case GroupEnd(id) => {
+                    assume id in groups;
+                    expect id in groups, "Group id was not seen before group end";
+                    var GroupStart := groups[id];
+                    groups := groups[id := (GroupStart.0, i)];
+                    states := states +[null];
+                    assume GroupStart.0 < i;
+                    for j := GroupStart.0 to i 
+                    {
+                        if(states[j] != null) {
+                            assert states[j] in states;
+                            states[j].groups := states[j].groups+{id};
+                        }
+                    }
+                }
+                case Concat => {
+                    // var e2 := pop(stack);
+                    assume |stack| > 1;
+                    expect |stack| > 1, "stack length was not greater than 1";
+                    var e2 := stack[|stack|-1];
+                    stack:=stack[..|stack|-1];
+                    var e1 := stack[|stack|-1];
+                    stack:=stack[..|stack|-1];
+                    assume forall i :: 0 <= i < |e1.out| ==>  fresh(OutSet(e1.out[i]));
+                    states := states +[null];
+                    patch(e1, e2);
+                    stack := stack + [FragC(e1.start, e2.out)];
+                }
+                case Alt => {
+                    assume |stack| > 1;
+                    expect |stack| > 1, "stack length was not greater than 1";
+                    var e2 := stack[|stack|-1];
+                    stack:=stack[..|stack|-1];
+                    var e1 := stack[|stack|-1];
+                    stack:=stack[..|stack|-1];
+                    var s := new State(sid, Split, e1.start, e2.start, false);
+                    s.origin := postfix[i];
+                    states := states+[s];
+                    sid := sid+1;
+                    stack := stack+[FragC(s, e1.out+e2.out)];
+                }
+                case Option => {
+                    assume |stack| > 0;
+                    expect |stack| > 0, "stack length was not greater than 1";
+                    var e1 := stack[|stack|-1];
+                    stack:=stack[..|stack|-1];
+                    var s := new State(sid, Split, e1.start, null, false);
+                    s.origin := postfix[i];
+                    states := states+[s];
+                    sid := sid+1;
+                    stack := stack+[FragC(s, e1.out+[Out1(s)])];
+                }
+                case Star => {
+                    assume |stack| > 0;
+                    expect |stack| > 0, "stack length was not greater than 1";
+                    var e1 := stack[|stack|-1];
+                    stack:=stack[..|stack|-1];
+                    var s := new State(sid, Split, e1.start, null, false);
+                    s.origin := postfix[i];
+                    states := states+[s];
+                    sid := sid+1;
+                    patch(e1, FragC(s,[]));
+                    stack := stack + [FragC(s, [Out1(s)])];
+                }
+                case Plus => {
+                    assume |stack| > 0;
+                    expect |stack| > 0, "stack length was not greater than 1";
+                    var e1 := stack[|stack|-1];
+                    stack:=stack[..|stack|-1];
+                    var s := new State(sid, Split, e1.start, null, false);
+                    s.origin := postfix[i];
+                    states := states+[s];
+                    sid := sid+1;
+                    patch(e1, FragC(s, []));
+                    stack := stack+[FragC(e1.start, [Out1(s)])];
+                }
+            }
+        }
+        assume |stack| > 0;
+        expect |stack| > 0, "stack length was not greater than 1";
+        var e := stack[|stack|-1];
+        var matchState := new State(sid, Match, null, null, false);
+        assume forall i :: 0 <= i < |e.out| ==>  fresh(OutSet(e.out[i]));
+        patch(e, FragC(matchState, []));
+        return e.start;
+    }
+
+    method ReMatch(re: string, targetString: string) returns (matches: bool, captures: seq<string>)
+
+    {
+        var postfix := re2post(re);
+        match postfix {
+            case Success(post) => {
+                var start := post2nfa([GroupStart(0)]+post+[GroupEnd(0)]);
+                matches := true;
+                captures := [];
+            }
+            case Failure(err) => {
+                print err;
+                matches := false;
+                captures := [];
+            }
+        }
     }
 
     method Main() {
@@ -122,5 +400,13 @@ module RegEx {
             case Failure(err) => print err;
         }
         
+    }
+
+    method test_re2post() {
+
+    }
+
+    method test_post2nfa() {
+
     }
 }
